theories/transparency/mealyproofs.v
@@ -143,8 +143,6 @@ Section outputs.
 Variable state : Type.
 Variable m : Mealy.t state.
 
-(** One step pushed onto the end: the analogue of Moore's [run_snoc]. Proved
-    by list induction; validated numerically before porting. *)
 Lemma outputs_snoc : forall w a q,
   outputs m q (w ++ [a])
   = outputs m q w ++ [m.(output _) (fold_left m.(transition _) w q) a].
@@ -264,7 +262,7 @@ Proof.
       destruct (enumerate_nth_error_pair _ (states state mealy) q_idx Hqb)
         as (q' & Hpair & Hnth).
       unfold sidx in Hq. apply index_of_nth_error in Hq.
-      rewrite Z.sub_0_r in Hq. rewrite Hq in Hnth. inversion Hnth; subst. exact Hpair. }
+      rewrite Z.sub_0_r in Hq. rewrite Hq in Hnth. inversion Hnth; subst. eauto. }
   assert (Hcol : nth_error (table_row state mealy state_eq_dec q) (Z.to_nat s_idx)
                  = Some (Init_int64 (Int64.repr (table_entry state mealy state_eq_dec q sym)))).
     { unfold table_row, sym_table. rewrite nth_error_map.
@@ -276,10 +274,8 @@ Proof.
   replace (Z.to_nat (q_idx * nsyms + s_idx))
     with (Z.to_nat q_idx * length s.enum + Z.to_nat s_idx)%nat
     by (unfold nsyms; lia).
-  rewrite nth_error_flat_map_uniform with (k := length s.enum) (x := (q_idx, q)).
-  - exact Hcol.
+  rewrite nth_error_flat_map_uniform with (k := length s.enum) (x := (q_idx, q)); eauto.
   - intros (qi & qq) _. apply table_row_length.
-  - exact Hrow.
   - lia.
 Qed.
 
@@ -308,7 +304,7 @@ Proof.
       destruct (enumerate_nth_error_pair _ (states state mealy) q_idx Hqb)
         as (q' & Hpair & Hnth).
       unfold sidx in Hq. apply index_of_nth_error in Hq.
-      rewrite Z.sub_0_r in Hq. rewrite Hq in Hnth. inversion Hnth; subst. exact Hpair. }
+      rewrite Z.sub_0_r in Hq. rewrite Hq in Hnth. inversion Hnth; subst. eauto. }
   assert (Hcol : nth_error (otable_row state mealy q) (Z.to_nat s_idx)
                  = Some (Init_int64 (Int64.repr (otable_entry state mealy q sym)))).
     { unfold otable_row, sym_table. rewrite nth_error_map.
@@ -320,10 +316,8 @@ Proof.
   replace (Z.to_nat (q_idx * nsyms + s_idx))
     with (Z.to_nat q_idx * length s.enum + Z.to_nat s_idx)%nat
     by (unfold nsyms; lia).
-  rewrite nth_error_flat_map_uniform with (k := length s.enum) (x := (q_idx, q)).
-  - exact Hcol.
+  rewrite nth_error_flat_map_uniform with (k := length s.enum) (x := (q_idx, q)); eauto.
   - intros (qi & qq) _. apply otable_row_length.
-  - exact Hrow.
   - lia.
 Qed.
 
@@ -391,6 +385,24 @@ Proof.
   rewrite Hdefs. right. now left.
 Qed.
 
+Lemma find_delta :
+  exists b,
+    Genv.find_symbol ge ids.(id_delta) = Some b /\
+    Genv.find_funct ge (Vptr b Ptrofs.zero) = Some (compile_delta state mealy ids).
+Proof.
+  assert (Hd : (prog_defmap p) ! (ids.(id_delta))
+               = Some (Gfun (compile_delta state mealy ids))).
+  { apply prog_defmap_norepet.
+      apply global_idents_norepet.
+    pose proof compile_program_defs as Hdefs.
+    change (AST.prog_defs p) with (prog_defs p).
+    rewrite Hdefs. right. right. now left. }
+  destruct (proj1 (Genv.find_def_symbol _ _ _) Hd) as (b & Hsym & Hdef).
+  exists b. split. eauto.
+  unfold Genv.find_funct. rewrite pred_dec_true by reflexivity.
+  now apply Genv.find_funct_ptr_iff.
+Qed.
+
 Lemma init_data_list_nth_load_int64 :
   forall (F V : Type) (ge' : Genv.t F V) b il n v m base_ofs,
   (forall id, In id il -> exists x, id = Init_int64 x) ->
@@ -451,7 +463,7 @@ Proof.
   destruct find_table as (b' & Hsym' & Hdef).
   assert (b' = b) by congruence. subst b'.
   assert (Hvi : Genv.find_var_info ge b = Some (compile_table state mealy state_eq_dec)).
-    { apply Genv.find_var_info_iff. exact Hdef. }
+    { apply Genv.find_var_info_iff. eauto. }
   destruct (Genv.init_mem_characterization _ _ Hvi Hinit)
     as (_ & _ & Hlsid & _).
   specialize (Hlsid eq_refl).
@@ -473,7 +485,7 @@ Proof.
   destruct find_otable as (b' & Hsym' & Hdef).
   assert (b' = b) by congruence. subst b'.
   assert (Hvi : Genv.find_var_info ge b = Some (compile_otable state mealy)).
-    { apply Genv.find_var_info_iff. exact Hdef. }
+    { apply Genv.find_var_info_iff. eauto. }
   destruct (Genv.init_mem_characterization _ _ Hvi Hinit)
     as (_ & _ & Hlsid & _).
   specialize (Hlsid eq_refl).
@@ -557,8 +569,10 @@ Proof.
     destruct Archi.ptr64; cbn; lia.
 Qed.
 
-(* delta is correct on valid indices *)
-Lemma compile_delta_correct :
+(* delta(q,a,out): write the output index through [out], return the successor
+   index. [b_o <> b_t/b_ot] keep the store from clobbering either table, so the
+   return still reads [table] from the post-store memory. *)
+Theorem compile_delta_correct :
   forall q sym q_idx s_idx next_idx o_idx b_o ofs_o b_t b_ot m,
   sidx q = Some q_idx ->
   symidx sym = Some s_idx ->
@@ -595,7 +609,7 @@ Proof.
   (* the write through [out] *)
   destruct (Mem.valid_access_store m Mint64 b_o ofs_o (Vlong (Int64.repr o_idx)))
     as (m' & Hstore).
-  { split; [| exact Halign]. intros z Hz. eapply Mem.perm_implies.
+  { split; [| eauto]. intros z Hz. eapply Mem.perm_implies.
       apply Hperm. cbn in Hz. lia.
     constructor. }
   exists m'. split. unfold Mem.storev. replace (Ptrofs.unsigned _) with ofs_o. assumption.
@@ -651,7 +665,7 @@ Proof.
                  --- eapply eval_Elvalue.
                        eapply eval_Evar_global.
                          apply PTree.gempty.
-                         exact Hbot.
+                         eauto.
                        eapply deref_loc_reference. reflexivity.
                  --- unfold table_index. econstructor.
                      +++ econstructor.
@@ -683,7 +697,7 @@ Proof.
                  change Ptrofs.zero with (Ptrofs.repr 0).
                  rewrite ptr_add_normalize by
                    (pose proof ptrofs_le_int64; unfold MC.nstates, MC.nsyms in *; nia).
-                 rewrite Z.add_0_l. exact Hloadot.
+                 rewrite Z.add_0_l. eauto.
            ++ cbn. unfold sem_cast, classify_cast, tlong. destruct Archi.ptr64; reflexivity.
            ++ (* assign_loc: the actual store to [b_o, ofs_o] *)
               eapply assign_loc_value with (chunk := Mint64).
@@ -697,7 +711,7 @@ Proof.
               ** eapply eval_Elvalue.
                    eapply eval_Evar_global.
                      apply PTree.gempty.
-                     exact Hbt.
+                     eauto.
                    eapply deref_loc_reference. reflexivity.
               ** unfold table_index. econstructor.
                  --- econstructor.
@@ -735,12 +749,12 @@ Proof.
       unfold tlong, sem_cast, classify_cast. now destruct Archi.ptr64.
     + reflexivity.
   - (* Mem.unchanged_on *)
-    eapply Mem.store_unchanged_on; [exact Hstore |].
-    intros i Hi [Hb | Hrange]; [now apply Hb |].
+    eapply Mem.store_unchanged_on; eauto.
+    intros i Hi [Hb | Hrange]; eauto.
     cbn [size_chunk] in *. lia.
 Qed.
 
-(* [delta] on out-of-range input writes [|O|] and returns [|Q|]. *)
+(* out-of-range input: write |O| through [out], return |Q|; reads no table *)
 Lemma compile_delta_sink :
   forall q_idx s_idx b_o ofs_o m,
   0 <= q_idx < Int64.modulus -> 0 <= s_idx < Int64.modulus ->
@@ -758,7 +772,7 @@ Proof.
   intros q_idx s_idx b_o ofs_o m Hq Hs Hoob Hperm Halign Hofs0 Hofsb.
   destruct (Mem.valid_access_store m Mint64 b_o ofs_o (Vlong (Int64.repr nouts)))
     as (m' & Hstore).
-  { split; [| exact Halign]. intros z Hz. eapply Mem.perm_implies.
+  { split; [| eauto]. intros z Hz. eapply Mem.perm_implies.
       apply Hperm. cbn in Hz. lia.
     constructor. }
   exists m'. split.
@@ -807,7 +821,7 @@ Proof.
     + cbn. split. discriminate.
       unfold tlong, sem_cast, classify_cast. now destruct Archi.ptr64.
     + reflexivity.
-  - eapply Mem.store_unchanged_on; [exact Hstore |].
+  - eapply Mem.store_unchanged_on; eauto.
     intros i Hi [Hb | Hrange]. now apply Hb.
     simpl size_chunk in Hi. lia.
 Qed.
@@ -826,21 +840,435 @@ Definition word_in_mem (m : mem) (b : block) (ofs : Z) (l : list Z) : Prop :=
     Mem.loadv Mint64 m (Vptr b (Ptrofs.repr (ofs + 8 * Z.of_nat n)))
       = Some (Vlong (Int64.repr i)).
 
-(* After [run(w, len, out)], the buffer [out] holds the [run_outputs] index
-   string, and only the buffer changed. *)
-Lemma compile_run_correct :
+Definition loop_frame (b_o b_out : block) (lo hi : Z) : block -> Z -> Prop :=
+  fun b o => b <> b_o /\ (b <> b_out \/ o < lo \/ hi <= o).
+
+Definition perms_eq (m m' : mem) : Prop :=
+  forall b ofs k pp, Mem.perm m b ofs k pp <-> Mem.perm m' b ofs k pp.
+
+Lemma perms_eq_refl : forall m, perms_eq m m.
+Proof. intros m b ofs k pp. reflexivity. Qed.
+
+Lemma perms_eq_trans : forall m1 m2 m3,
+  perms_eq m1 m2 -> perms_eq m2 m3 -> perms_eq m1 m3.
+Proof.
+  intros m1 m2 m3 H12 H23 b ofs k pp.
+  etransitivity. apply H12. apply H23.
+Qed.
+
+Lemma perms_eq_store : forall chunk m b ofs v m',
+  Mem.store chunk m b ofs v = Some m' -> perms_eq m m'.
+Proof.
+  intros chunk m b ofs v m' Hst b' ofs' k pp. split; intro Hp'.
+  - eapply Mem.perm_store_1; eauto.
+  - eapply Mem.perm_store_2; eauto.
+Qed.
+
+Lemma run_loop_correct :
+  forall w2 w1 l2 lo2 e le b_w ofs_w b_out ofs_out b_o b_t b_ot m,
+  sym_indices w2 l2 ->
+  Forall2 (fun o i => oidx o = Some i)
+          (outputs mealy (Mealy.run mealy w1) w2) lo2 ->
+  (forall n i, nth_error l2 n = Some i ->
+     Mem.loadv Mint64 m (Vptr b_w (Ptrofs.repr
+        (ofs_w + 8 * Z.of_nat (length w1 + n)))) = Some (Vlong (Int64.repr i))) ->
+  Genv.find_symbol ge ids.(id_table)  = Some b_t ->
+  Genv.find_symbol ge ids.(id_otable) = Some b_ot ->
+  (forall k v, nth_error (table_init state mealy state_eq_dec) (Z.to_nat k)
+       = Some (Init_int64 v) -> 0 <= k < nstates * nsyms ->
+       Mem.loadv Mint64 m (Vptr b_t (Ptrofs.repr (8*k))) = Some (Vlong v)) ->
+  (forall k v, nth_error (otable_init state mealy) (Z.to_nat k)
+       = Some (Init_int64 v) -> 0 <= k < nstates * nsyms ->
+       Mem.loadv Mint64 m (Vptr b_ot (Ptrofs.repr (8*k))) = Some (Vlong v)) ->
+  e ! (id_o ids) = Some (b_o, tlong) ->
+  le ! (id_i ids)   = Some (Vlong (Int64.repr (Z.of_nat (length w1)))) ->
+  (exists qi, sidx (Mealy.run mealy w1) = Some qi
+     /\ le ! (id_q ids) = Some (Vlong (Int64.repr qi))) ->
+  le ! (id_w ids)   = Some (Vptr b_w   (Ptrofs.repr ofs_w)) ->
+  le ! (id_out ids) = Some (Vptr b_out (Ptrofs.repr ofs_out)) ->
+  le ! (id_len ids) = Some (Vlong (Int64.repr (Z.of_nat (length w1 + length w2)))) ->
+  e ! (id_delta ids) = None ->
+  b_w <> b_t -> b_w <> b_ot -> b_out <> b_t -> b_out <> b_ot -> b_w <> b_out ->
+  b_o <> b_t -> b_o <> b_ot -> b_o <> b_out -> b_o <> b_w ->
+  Mem.range_perm m b_o 0 8 Cur Writable ->
+  Mem.range_perm m b_out (ofs_out + 8 * Z.of_nat (length w1))
+     (ofs_out + 8 * Z.of_nat (length w1 + length w2)) Cur Writable ->
+  (align_chunk Mint64 | ofs_out) ->
+  0 <= ofs_w -> 0 <= ofs_out ->
+  Z.of_nat (length w1 + length w2) < Int64.modulus ->
+  ofs_w   + 8 * Z.of_nat (length w1 + length w2) < Ptrofs.modulus ->
+  ofs_out + 8 * Z.of_nat (length w1 + length w2) < Ptrofs.modulus ->
+  exists m' le',
+    exec_stmt function_entry2 ge e le m (run_loop ids) E0 le' m' Out_normal /\
+    buf_in_mem m' b_out (ofs_out + 8 * Z.of_nat (length w1)) lo2 /\
+    perms_eq m m' /\
+    Mem.unchanged_on
+      (loop_frame b_o b_out (ofs_out + 8 * Z.of_nat (length w1))
+                            (ofs_out + 8 * Z.of_nat (length w1 + length w2))) m m'.
+Proof.
+  induction w2 as [| a w2' IH];
+    intros w1 l2 lo2 e le b_w ofs_w b_out ofs_out b_o b_t b_ot m
+      Hsym Hout Hword Hbt Hbot Htload Hotload Ho Hi Hq Hw Hout' Hlen Hdelta_id
+      Hbwt Hbwot Hboutt Hboutot Hbwo
+      Hbot_t Hbot_ot Hbo_out Hbo_w
+      Hperm_o Hperm_out Halign Hofsw Hofsout
+      Hlenmod Hwmod Houtmod.
+
+  - cbn [length outputs] in *. rewrite Nat.add_0_r in *.
+    inversion Hout; subst; clear Hout.
+    exists m, le. split; [| split; [| split]].
+    + eapply exec_Sloop_stop1; [| constructor].
+      unfold run_loop, MC.run_body.
+      eapply exec_Sseq_2; [| discriminate].
+      eapply exec_Sifthenelse with (b := false).
+      * econstructor; [ econstructor; eauto | econstructor; eauto |].
+        cbn. unfold sem_cmp, classify_cmp, tlong, sem_binarith, sem_cast,
+                   classify_cast, classify_binarith. cbn.
+        destruct Archi.ptr64; cbn; unfold Val.of_bool, Int64.ltu;
+          rewrite !Int64.unsigned_repr by (unfold Int64.max_unsigned; lia);
+          rewrite zlt_false by lia; reflexivity.
+      * apply bool_val_zero_int.
+      * constructor.
+    + intros n i Hn. now destruct n.
+    + apply perms_eq_refl.
+    + apply Mem.unchanged_on_refl.
+
+  - inversion Hsym as [| a0 si w0 l2' Hsi Hsym' [Ea El]]; subst; clear Hsym.
+    cbn [outputs] in Hout.
+    set (qw := Mealy.run mealy w1) in *.
+    inversion Hout as [| o0 oi outs lo2' Hoi Hout'' [Eo Elo]]; subst; clear Hout.
+    destruct Hq as (qi & Hqi & Hqle).
+
+    (* the index of the successor state *)
+    destruct (sidx_run (w1 ++ [a])) as (ni & Hni).
+    assert (Hnext : sidx (mealy.(transition _) qw a) = Some ni).
+    { rewrite <- Hni. unfold qw, Mealy.run. now rewrite fold_left_app. }
+
+    assert (Hqib : 0 <= qi < nstates) by
+      (unfold sidx, nstates, MC.nstates in *; apply index_of_bounds in Hqi; lia).
+    assert (Hsib : 0 <= si < nsyms) by
+      (unfold symidx, nsyms in *; apply index_of_bounds in Hsi; lia).
+    assert (Hcell : 0 <= qi * nsyms + si < nstates * nsyms) by
+      (clear - Hqib Hsib;
+       unfold nstates, nsyms in *; nia).
+
+    (* the two table cells [delta] will read, at the current memory [m] *)
+    assert (Hloadt :
+      Mem.loadv Mint64 m (Vptr b_t (Ptrofs.repr (8 * (qi * nsyms + si))))
+        = Some (Vlong (Int64.repr ni))).
+    { apply Htload with (k := qi * nsyms + si); [| eauto].
+      erewrite table_entry_correct by eauto.
+      do 2 f_equal. now erewrite table_entry_sidx by eauto. }
+    assert (Hloadot :
+      Mem.loadv Mint64 m (Vptr b_ot (Ptrofs.repr (8 * (qi * nsyms + si))))
+        = Some (Vlong (Int64.repr oi))).
+    { apply Hotload with (k := qi * nsyms + si); [| eauto].
+      erewrite otable_entry_correct by eauto.
+      do 2 f_equal. now erewrite otable_entry_oidx by eauto. }
+
+    assert (H8lt : 0 + 8 < Ptrofs.modulus).
+    { unfold Ptrofs.modulus, Ptrofs.wordsize, Wordsize_Ptrofs.wordsize, two_power_nat.
+      destruct Archi.ptr64; cbn; lia. }
+
+    destruct (compile_delta_correct
+                qw a qi si ni oi b_o 0 b_t b_ot m
+                Hqi Hsi Hnext Hoi Hbt Hbot Hloadt Hloadot
+                Hperm_o (Z.divide_0_r _) (Z.le_refl 0) H8lt Hbot_t Hbot_ot)
+      as (m1 & Hstore_o & Hdelta & Hunch1).
+    assert (Hstore_o' : Mem.store Mint64 m b_o 0 (Vlong (Int64.repr oi)) = Some m1).
+    { unfold Mem.storev in Hstore_o.
+      rewrite Ptrofs.unsigned_repr in Hstore_o
+        by (unfold Ptrofs.max_unsigned; pose proof Ptrofs.modulus_pos; lia).
+      eauto. }
+
+    (* the symbol w[i] sits at ofs_w + 8|w1| and survives delta's write *)
+    assert (Hwi :
+      Mem.loadv Mint64 m (Vptr b_w (Ptrofs.repr (ofs_w + 8 * Z.of_nat (length w1))))
+        = Some (Vlong (Int64.repr si))).
+    { specialize (Hword O si eq_refl). now rewrite Nat.add_0_r in Hword. }
+
+    assert (Hperm_out1 : Mem.range_perm m1 b_out
+              (ofs_out + 8 * Z.of_nat (length w1))
+              (ofs_out + 8 * Z.of_nat (length w1) + 8) Cur Writable).
+    { intros z Hz. eapply Mem.perm_store_1; eauto.
+      apply Hperm_out. cbn [length] in *. rewrite Nat.add_succ_r. lia. }
+    destruct (Mem.valid_access_store m1 Mint64 b_out
+                (ofs_out + 8 * Z.of_nat (length w1)) (Vlong (Int64.repr oi)))
+      as (m2 & Hstore_out).
+    { split.
+      - intros z Hz. eapply Mem.perm_implies; [| constructor].
+        apply Hperm_out1. cbn [size_chunk] in Hz. lia.
+      - apply Z.divide_add_r; eauto.
+        apply Z.divide_mul_l. apply Z.divide_refl. }
+
+    (* permissions are untouched by both stores *)
+    assert (Hpe2 : perms_eq m m2).
+    { eapply perms_eq_trans;
+        [ eapply perms_eq_store; eauto
+        | eapply perms_eq_store; eauto ]. }
+
+    (* the frame for this single iteration *)
+    assert (Hunch2 : Mem.unchanged_on
+              (loop_frame b_o b_out (ofs_out + 8 * Z.of_nat (length w1))
+                                    (ofs_out + 8 * Z.of_nat (length w1) + 8)) m m2).
+    { eapply Mem.unchanged_on_trans.
+      - eapply Mem.unchanged_on_implies; eauto.
+        intros b o (Hbo & _) _. now left.
+      - eapply Mem.store_unchanged_on; eauto.
+        intros z Hz (_ & [Hb | [Hlt | Hge]]); 
+          [congruence | cbn [size_chunk] in Hz; lia | cbn [size_chunk] in Hz; lia]. }
+
+    assert (Hword2 : forall n j, nth_error l2' n = Some j ->
+       Mem.loadv Mint64 m2 (Vptr b_w (Ptrofs.repr
+          (ofs_w + 8 * Z.of_nat (length (w1 ++ [a]) + n))))
+          = Some (Vlong (Int64.repr j))).
+    { intros n j Hn. unfold Mem.loadv in *.
+      erewrite Mem.load_unchanged_on; [reflexivity | eauto | |].
+      - intros z _. split; [congruence | now left].
+      - rewrite length_app. cbn [length]. rewrite Nat.add_1_r.
+        specialize (Hword (S n) j).
+        replace (S (length w1) + n)%nat with (length w1 + S n)%nat by lia.
+        apply Hword. cbn [nth_error]. eauto. }
+    assert (Htload2 : forall k v,
+       nth_error (table_init state mealy state_eq_dec) (Z.to_nat k)
+         = Some (Init_int64 v) -> 0 <= k < nstates * nsyms ->
+       Mem.loadv Mint64 m2 (Vptr b_t (Ptrofs.repr (8*k))) = Some (Vlong v)).
+    { intros k v Hk Hkb. unfold Mem.loadv in *.
+      erewrite Mem.load_unchanged_on; [reflexivity | eauto | | now apply Htload].
+      intros z _. split; [congruence | now left]. }
+    assert (Hotload2 : forall k v,
+       nth_error (otable_init state mealy) (Z.to_nat k)
+         = Some (Init_int64 v) -> 0 <= k < nstates * nsyms ->
+       Mem.loadv Mint64 m2 (Vptr b_ot (Ptrofs.repr (8*k))) = Some (Vlong v)).
+    { intros k v Hk Hkb. unfold Mem.loadv in *.
+      erewrite Mem.load_unchanged_on; [reflexivity | eauto | | now apply Hotload].
+      intros z _. split; [congruence | now left]. }
+    assert (Hperm_o2 : Mem.range_perm m2 b_o 0 8 Cur Writable).
+    { intros z Hz. apply Hpe2. now apply Hperm_o. }
+    assert (Hperm_out2 : Mem.range_perm m2 b_out
+              (ofs_out + 8 * Z.of_nat (length (w1 ++ [a])))
+              (ofs_out + 8 * Z.of_nat (length (w1 ++ [a]) + length w2')) Cur Writable).
+    { intros z Hz. apply Hpe2. apply Hperm_out.
+      rewrite length_app in Hz. cbn [length] in *.
+      rewrite Nat.add_1_r, Nat.add_succ_r in *. lia. }
+
+    (* the temp env after this iteration *)
+    set (le2 := PTree.set (id_i ids)
+                  (Vlong (Int64.repr (Z.of_nat (length w1) + 1)))
+                  (PTree.set (id_q ids) (Vlong (Int64.repr ni)) le)) in *.
+
+    edestruct (IH (w1 ++ [a]) l2' lo2' e le2
+                 b_w ofs_w b_out ofs_out b_o b_t b_ot m2)
+      as (m' & le' & Hexec' & Hbuf' & Hpe' & Hunch').
+    all: subst le2; eauto.
+    + (* the outputs of w2' start from run (w1 ++ [a]) *)
+      unfold Mealy.run in *. now rewrite fold_left_app.
+    + (* i = |w1 ++ [a]| *)
+      rewrite PTree.gss. rewrite length_app. cbn [length]. do 3 f_equal. lia.
+    + (* q = sidx (run (w1 ++ [a])) *)
+      exists ni. split; eauto.
+      rewrite PTree.gso by (cbv [ids alloc_idents id_i id_q]; lia).
+      apply PTree.gss.
+    + rewrite PTree.gso by (cbv [ids alloc_idents id_w id_i]; lia).
+      rewrite PTree.gso by (cbv [ids alloc_idents id_w id_q]; lia). eauto.
+    + rewrite PTree.gso by (cbv [ids alloc_idents id_out id_i]; lia).
+      rewrite PTree.gso by (cbv [ids alloc_idents id_out id_q]; lia). eauto.
+    + rewrite PTree.gso by (cbv [ids alloc_idents id_len id_i]; lia).
+      rewrite PTree.gso by (cbv [ids alloc_idents id_len id_q]; lia).
+      rewrite Hlen. do 3 f_equal. rewrite length_app. cbn [length]. lia.
+    + rewrite length_app in *. cbn [length] in *.
+      rewrite Nat.add_1_r, Nat.add_succ_r in *. lia.
+    + rewrite length_app in *. cbn [length] in *.
+      rewrite Nat.add_1_r, Nat.add_succ_r in *. lia.
+    + rewrite length_app in *. cbn [length] in *.
+      rewrite Nat.add_1_r, Nat.add_succ_r in *. lia.
+
+    + destruct find_delta as (b_d & Hdsym & Hdfun).
+      exists m', le'. split; [| split; [| split]].
+      * (* one turn of the loop, then the rest *)
+        change E0 with (E0 ** E0 ** E0).
+        eapply exec_Sloop_loop with (out1 := Out_normal); revgoals.
+        -- eauto.
+        -- constructor.
+        -- constructor.
+        -- (* the body: guard; q = delta(q, w[i], &o); out[i] = o; i++ *)
+           unfold MC.run_body.
+           change E0 with (E0 ** E0).
+           eapply exec_Sseq_1.
+           ++ (* the guard is true *)
+              eapply exec_Sifthenelse with (b := true).
+              ** econstructor; [ econstructor; eauto | econstructor; eauto |].
+                 cbn. unfold sem_cmp, classify_cmp, tlong, sem_binarith, sem_cast,
+                            classify_cast, classify_binarith. cbn.
+                 destruct Archi.ptr64; cbn; unfold Val.of_bool, Int64.ltu;
+                   rewrite !Int64.unsigned_repr by
+                     (unfold Int64.max_unsigned; cbn [length] in *; lia);
+                   rewrite zlt_true by (cbn [length]; lia); reflexivity.
+              ** apply bool_val_one_int.
+              ** constructor.
+           ++ change E0 with (E0 ** E0).
+              eapply exec_Sseq_1.
+              ** (* q = delta(q, w[i], &o) *)
+                 eapply exec_Scall with
+                   (vargs := [Vlong (Int64.repr qi); Vlong (Int64.repr si);
+                              Vptr b_o Ptrofs.zero]).
+                 --- reflexivity.
+                 --- eapply eval_Elvalue.
+                       eapply eval_Evar_global; eauto.
+                     eapply deref_loc_reference. reflexivity.
+                 --- (* the three arguments *)
+                     econstructor.
+                     +++ econstructor. eauto.
+                     +++ cbn. unfold sem_cast, classify_cast, tlong.
+                         now destruct Archi.ptr64.
+                     +++ econstructor.
+                         *** eapply eval_Elvalue.
+                             ---- econstructor. econstructor.
+                                  ++++ econstructor. eauto.
+                                  ++++ econstructor. eauto.
+                                  ++++ cbn. unfold sem_add, classify_add, w_type, tlong. cbn.
+                                       destruct Archi.ptr64 eqn:E; [| discriminate].
+                                       unfold sem_add_ptr_long. cbn. do 3 f_equal.
+                             ---- eapply deref_loc_value with (chunk := Mint64); eauto.
+                                  rewrite ptr_add_normalize by lia. apply Hwi.
+                         *** cbn. unfold sem_cast, classify_cast, tlong.
+                             now destruct Archi.ptr64.
+                         *** econstructor.
+                             ---- econstructor. econstructor. eauto.
+                             ---- cbn. unfold sem_cast, classify_cast, tlptr. cbn.
+                                  now destruct Archi.ptr64.
+                             ---- econstructor.
+                 --- unfold Genv.find_funct in Hdfun |- *. eauto.
+                 --- reflexivity.
+                 --- eauto.
+              ** change E0 with (E0 ** E0).
+                 eapply exec_Sseq_1.
+                 --- (* out[i] = o *)
+                     econstructor.
+                     +++ (* lvalue out + i *)
+                         econstructor. econstructor.
+                         *** econstructor. cbn - [Pos.add].
+                             rewrite PTree.gso
+                               by (cbv [ids alloc_idents id_out id_q]; lia).
+                             eauto.
+                         *** econstructor. cbn - [Pos.add].
+                             rewrite PTree.gso
+                               by (cbv [ids alloc_idents id_i id_q]; lia).
+                             eauto.
+                         *** cbn. unfold sem_add, classify_add, tlptr, tlong. cbn.
+                             destruct Archi.ptr64 eqn:E; [| discriminate].
+                             unfold sem_add_ptr_long. cbn. do 3 f_equal.
+                     +++ (* rvalue: the scratch [o], read back out of m1 *)
+                         eapply eval_Elvalue.
+                         *** econstructor. eauto.
+                         *** eapply deref_loc_value with (chunk := Mint64).
+                               reflexivity.
+                             cbn [Mem.loadv]. rewrite Ptrofs.unsigned_zero.
+                             rewrite (Mem.load_store_same _ _ _ _ _ _ Hstore_o').
+                             reflexivity.
+                     +++ cbn. unfold sem_cast, classify_cast, tlong.
+                         now destruct Archi.ptr64.
+                     +++ eapply assign_loc_value with (chunk := Mint64).
+                           reflexivity.
+                         cbn [Mem.storev]. rewrite ptr_add_normalize by lia.
+                         rewrite Ptrofs.unsigned_repr by
+                          (unfold Ptrofs.max_unsigned, nsyms, nstates in *; lia).
+                         apply Hstore_out.
+                 --- (* i++ *)
+                     econstructor. econstructor.
+                     +++ econstructor. cbn - [Pos.add].
+                         rewrite PTree.gso by (cbv [ids alloc_idents id_i id_q]; lia).
+                         eauto.
+                     +++ econstructor.
+                     +++ cbn. unfold sem_binarith, sem_cast, classify_cast,
+                                classify_binarith, tlong. cbn.
+                         destruct Archi.ptr64; cbn; do 2 f_equal;
+                           rewrite add_repr_in_range;
+                           solve [ reflexivity
+                                 | unfold Int64.max_unsigned;
+                                   cbn [length] in *; rewrite Nat.add_succ_r in *; lia ].
+      * (* buf_in_mem for [oi :: lo2'] *)
+        intros n j Hn. destruct n as [| n'].
+        -- (* the entry just stored, preserved across the recursive call *)
+           cbn [nth_error] in Hn. inversion Hn; subst j; clear Hn.
+           cbn [Z.of_nat]. rewrite Z.mul_0_r, Z.add_0_r.
+           unfold Mem.loadv.
+           erewrite Mem.load_unchanged_on; [| eauto | |].
+           ++ reflexivity.
+           ++ intros z Hz. split. congruence. right. left.
+              rewrite length_app. cbn [length]. rewrite Nat.add_1_r.
+              cbn [size_chunk] in Hz.
+              rewrite Ptrofs.unsigned_repr in Hz. lia.
+              unfold Ptrofs.max_unsigned, nstates, nsyms in *.
+              lia.
+           ++ pose proof (Mem.load_store_same _ _ _ _ _ _ Hstore_out).
+              rewrite Ptrofs.unsigned_repr by
+                (unfold Ptrofs.max_unsigned, nstates, nsyms in *; lia).
+              apply H.
+        -- (* the rest, from the recursive call *)
+           cbn [nth_error] in Hn.
+           specialize (Hbuf' n' j Hn).
+           rewrite length_app in Hbuf'. cbn [length] in Hbuf'.
+           rewrite Nat.add_1_r in Hbuf'.
+           replace (ofs_out + 8 * Z.of_nat (length w1) + 8 * Z.of_nat (S n'))
+             with (ofs_out + 8 * Z.of_nat (S (length w1)) + 8 * Z.of_nat n')
+             by (rewrite !Nat2Z.inj_succ; lia).
+           eauto.
+      * (* permissions *) eapply perms_eq_trans; [eauto | eauto].
+      * (* the composite frame *)
+        eapply Mem.unchanged_on_trans.
+        -- eapply Mem.unchanged_on_implies; eauto.
+           intros b o (Hbo & Hrest) _. split; eauto.
+           destruct Hrest as [Hb | [Hlt | Hge]]; [now left | now right; left |].
+           right. right. cbn [length] in Hge. rewrite Nat.add_succ_r in Hge. lia.
+        -- eapply Mem.unchanged_on_implies; eauto.
+           intros b o (Hbo & Hrest) _. split; eauto.
+           destruct Hrest as [Hb | [Hlt | Hge]]; [now left | |].
+           ++ right. left. rewrite length_app. cbn [length]. rewrite Nat.add_1_r.
+              rewrite Nat2Z.inj_succ. lia.
+           ++ right. right. rewrite length_app. cbn [length] in *.
+              rewrite Nat.add_1_r, Nat.add_succ_r in *. lia.
+Qed.
+
+Lemma elements_singleton : forall (A : Type) (i : positive) (v : A),
+  PTree.elements (PTree.set i v (PTree.empty A)) = [(i, v)].
+Proof.
+  intros A i v.
+  assert (Hin : In (i, v) (PTree.elements (PTree.set i v (PTree.empty A))))
+    by (apply PTree.elements_correct; apply PTree.gss).
+  assert (Hall : forall x, In x (PTree.elements (PTree.set i v (PTree.empty A)))
+                   -> x = (i, v)).
+  { intros (j & w) Hj. apply PTree.elements_complete in Hj.
+    destruct (peq j i) as [-> | Hne].
+    - rewrite PTree.gss in Hj. now inversion Hj.
+    - rewrite PTree.gso in Hj by eauto.
+      rewrite PTree.gempty in Hj. discriminate. }
+  pose proof (PTree.elements_keys_norepet (PTree.set i v (PTree.empty A))) as Hnr.
+  destruct (PTree.elements (PTree.set i v (PTree.empty A)))
+    as [| x [| y tl]] eqn:E.
+  - destruct Hin.
+  - now rewrite (Hall x (or_introl eq_refl)).
+  - exfalso.
+    rewrite (Hall x (or_introl eq_refl)) in Hnr.
+    rewrite (Hall y (or_intror (or_introl eq_refl))) in Hnr.
+    cbn in Hnr. inversion Hnr as [| ? ? Hni ?]; subst. apply Hni. now left.
+Qed.
+
+(* run: the output buffer ends holding the run's outputs *)
+Theorem compile_run_correct :
   forall w l lo b_w ofs_w b_out ofs_out b_t b_ot m,
   sym_indices w l ->
   Forall2 (fun o i => oidx o = Some i) (run_outputs mealy w) lo ->
   word_in_mem m b_w ofs_w l ->
   Genv.find_symbol ge ids.(id_table) = Some b_t ->
   Genv.find_symbol ge ids.(id_otable) = Some b_ot ->
-  Mem.unchanged_on (fun b _ => b <> b_t /\ b <> b_ot) m0 m ->
   (forall k v, nth_error (table_init state mealy state_eq_dec) (Z.to_nat k) = Some (Init_int64 v) ->
      0 <= k < nstates * nsyms -> Mem.loadv Mint64 m (Vptr b_t (Ptrofs.repr (8 * k))) = Some (Vlong v)) ->
   (forall k v, nth_error (otable_init state mealy) (Z.to_nat k) = Some (Init_int64 v) ->
      0 <= k < nstates * nsyms -> Mem.loadv Mint64 m (Vptr b_ot (Ptrofs.repr (8 * k))) = Some (Vlong v)) ->
   b_w <> b_t -> b_w <> b_ot -> b_out <> b_t -> b_out <> b_ot ->
+  Mem.valid_block m b_w -> Mem.valid_block m b_out ->
+  Mem.valid_block m b_t -> Mem.valid_block m b_ot ->
   Mem.range_perm m b_out ofs_out (ofs_out + 8 * Z.of_nat (length w)) Cur Writable ->
   (align_chunk Mint64 | ofs_out) ->
   0 <= ofs_w -> 0 <= ofs_out ->
@@ -856,7 +1284,148 @@ Lemma compile_run_correct :
     buf_in_mem m' b_out ofs_out lo /\
     Mem.unchanged_on (fun b _ => b <> b_out) m m'.
 Proof.
-Admitted.
+  intros w l lo b_w ofs_w b_out ofs_out b_t b_ot m
+    Hsym Hout Hword Hbt Hbot Htload Hotload
+    Hbwt Hbwot Hboutt Hboutot Hvw Hvout Hvt Hvot
+    Hperm_out Halign Hofsw Hofsout Hbwo Hlenmod Hwmod Houtmod.
+
+  destruct (Mem.alloc m 0 (sizeof ge tlong)) as (m1 & b_o) eqn:Halloc.
+  set (e := PTree.set (id_o ids) (b_o, tlong) (PTree.empty (block * type))).
+
+  assert (Hfresh : ~ Mem.valid_block m b_o)
+    by (eapply Mem.fresh_block_alloc; eauto).
+  assert (Hbo_w   : b_o <> b_w)   by (intro; subst; contradiction).
+  assert (Hbo_out : b_o <> b_out) by (intro; subst; contradiction).
+  assert (Hbo_t   : b_o <> b_t)   by (intro; subst; contradiction).
+  assert (Hbo_ot  : b_o <> b_ot)  by (intro; subst; contradiction).
+
+  assert (Hunch_alloc : forall P, Mem.unchanged_on P m m1)
+    by (intro P; eapply Mem.alloc_unchanged_on; eauto).
+
+  assert (Hword1 : forall n i, nth_error l n = Some i ->
+     Mem.loadv Mint64 m1 (Vptr b_w (Ptrofs.repr
+        (ofs_w + 8 * Z.of_nat (0 + n)))) = Some (Vlong (Int64.repr i))).
+  { intros n i Hn. cbn [Nat.add]. unfold Mem.loadv in *.
+    erewrite Mem.load_unchanged_on;
+      [reflexivity | apply Hunch_alloc | intros; exact I | now apply Hword]. }
+  assert (Htload1 : forall k v,
+     nth_error (table_init state mealy state_eq_dec) (Z.to_nat k) = Some (Init_int64 v) ->
+     0 <= k < nstates * nsyms ->
+     Mem.loadv Mint64 m1 (Vptr b_t (Ptrofs.repr (8*k))) = Some (Vlong v)).
+  { intros k v Hk Hkb. unfold Mem.loadv in *.
+    erewrite Mem.load_unchanged_on;
+      [reflexivity | apply Hunch_alloc | intros; exact I | now apply Htload]. }
+  assert (Hotload1 : forall k v,
+     nth_error (otable_init state mealy) (Z.to_nat k) = Some (Init_int64 v) ->
+     0 <= k < nstates * nsyms ->
+     Mem.loadv Mint64 m1 (Vptr b_ot (Ptrofs.repr (8*k))) = Some (Vlong v)).
+  { intros k v Hk Hkb. unfold Mem.loadv in *.
+    erewrite Mem.load_unchanged_on;
+      [reflexivity | apply Hunch_alloc | intros; exact I | now apply Hotload]. }
+  assert (Hperm_out1 : Mem.range_perm m1 b_out ofs_out
+            (ofs_out + 8 * Z.of_nat (0 + length w)) Cur Writable).
+  { intros z Hz. eapply Mem.perm_alloc_1; eauto. }
+  assert (Hperm_o1 : Mem.range_perm m1 b_o 0 8 Cur Writable).
+  { intros z Hz. eapply Mem.perm_implies.
+      eapply Mem.perm_alloc_2; eauto. constructor. }
+
+  (* temp env *)
+  set (le0 := PTree.set (id_out ids) (Vptr b_out (Ptrofs.repr ofs_out))
+               (PTree.set (id_len ids) (Vlong (Int64.repr (Z.of_nat (length w))))
+                 (PTree.set (id_w ids) (Vptr b_w (Ptrofs.repr ofs_w))
+                   (create_undef_temps
+                      [(ids.(id_i), tlong); (ids.(id_q), tlong)])))).
+  set (le1 := PTree.set (id_q ids)
+                (Vlong (Int64.repr (q0_index state mealy state_eq_dec)))
+                (PTree.set (id_i ids) (Vlong (Int64.repr 0)) le0)).
+
+  (* loop *)
+  edestruct (run_loop_correct w [] l lo e le1
+               b_w ofs_w b_out ofs_out b_o b_t b_ot m1)
+    as (m2 & le' & Hexec & Hbuf & Hpe & Hunch_loop).
+  all: eauto.
+  + (* o = b_o *)
+    subst e. now rewrite PTree.gss.
+  + (* i = 0 *)
+    subst le1. rewrite PTree.gso by (cbv [ids alloc_idents id_i id_q]; lia).
+    apply PTree.gss.
+  + (* q = q0 *)
+    exists (q0_index state mealy state_eq_dec). split.
+      cbn [Mealy.run fold_left]. apply q0_index_correct.
+    subst le1. apply PTree.gss.
+  + (* w = &ofs_w *)
+    subst le1. rewrite PTree.gso by (cbv [ids alloc_idents id_w id_q]; lia).
+    rewrite PTree.gso by (cbv [ids alloc_idents id_w id_i]; lia).
+    subst le0. rewrite PTree.gso by (cbv [ids alloc_idents id_w id_out]; lia).
+    rewrite PTree.gso by (cbv [ids alloc_idents id_w id_len]; lia).
+    now rewrite PTree.gss.
+  + subst le1. rewrite PTree.gso by (cbv [ids alloc_idents id_out id_q]; lia).
+    rewrite PTree.gso by (cbv [ids alloc_idents id_out id_i]; lia).
+    subst le0. now rewrite PTree.gss.
+  + subst le1. rewrite PTree.gso by (cbv [ids alloc_idents id_len id_q]; lia).
+    rewrite PTree.gso by (cbv [ids alloc_idents id_len id_i]; lia).
+    subst le0. rewrite PTree.gso by (cbv [ids alloc_idents id_len id_out]; lia).
+    now rewrite PTree.gss.
+  + subst e. rewrite PTree.gso by (cbv [ids alloc_idents id_o id_delta]; lia).
+    apply PTree.gempty.
+  + cbn [length Z.of_nat]. rewrite Z.mul_0_r, Nat.add_0_l, Z.add_0_r. assumption.
+  + (* return *)
+    cbn [length Z.of_nat] in Hbuf. rewrite Z.mul_0_r, Z.add_0_r in Hbuf.
+    assert (Hfree : exists m3, Mem.free m2 b_o 0 8 = Some m3).
+    { pose proof (Mem.range_perm_free m2 b_o 0 8). destruct X.
+        intros z Hz. apply Hpe. eapply Mem.perm_alloc_2; eassumption.
+      now exists x. }
+    destruct Hfree as (m3 & Hfree).
+    assert (Hblocks : blocks_of_env ge e = [(b_o, 0, 8)]).
+    { unfold blocks_of_env, e. rewrite elements_singleton. reflexivity. }
+    exists m3. split; [| split].
+    * (* the call itself *)
+      eapply eval_funcall_internal with (e := e) (le1 := le0) (m1 := m1).
+      -- (* function_entry2 *)
+         econstructor; cbn - [Pos.add].
+         ++ repeat constructor. now intro.
+         ++ repeat constructor; cbn - [Pos.add]; intro Hin;
+              repeat (destruct Hin as [Hin|Hin]; [lia|]); contradiction.
+         ++ repeat intro. cbn - [Pos.add] in *.
+            repeat (destruct H as [H|H]; subst; try contradiction);
+            repeat (destruct H0 as [H0|H0]; subst; try contradiction); lia.
+         ++ econstructor; [eauto | constructor].
+         ++ reflexivity.
+      -- (* the body: prologue then loop *)
+         unfold compile_run. cbn [fn_body].
+         change E0 with (E0 ** E0).
+         eapply exec_Sseq_1.
+         ++ (* i := 0; q := q0 *)
+            change E0 with (E0 ** E0).
+            eapply exec_Sseq_1.
+            ** econstructor. econstructor.
+            ** econstructor. unfold compiled_q0. econstructor.
+         ++ eauto.
+      -- (* the outcome of a void function that falls off the end *)
+         cbn. auto.
+      -- rewrite Hblocks. cbn [Mem.free_list]. now rewrite Hfree.
+    * intros n i Hn. specialize (Hbuf n i Hn).
+      unfold Mem.loadv in *. erewrite Mem.load_free; eauto.
+    * apply (Mem.unchanged_on_implies
+               (fun b _ => b <> b_out /\ Mem.valid_block m b)).
+      -- eapply Mem.unchanged_on_trans; [| eapply Mem.unchanged_on_trans].
+         ++ (* m -> m1 : allocation changes nothing already present *) 
+            eapply Mem.unchanged_on_implies.
+              eapply Mem.alloc_unchanged_on; eauto.
+            intros b ofs Hb _. exact I.
+         ++ (* m1 -> m2 : the loop's frame, weakened using freshness of b_o *)
+            eapply Mem.unchanged_on_implies; eauto.
+            intros b ofs (Hbout & Hvb) _. split.
+              intro; subst b; contradiction.
+            now left.
+         ++ (* m2 -> m3 : the free touches only b_o, which is not valid in m *)
+            eapply Mem.unchanged_on_implies.
+              eapply (Mem.free_unchanged_on
+                        (fun b _ => b <> b_out /\ Mem.valid_block m b)); eauto.
+              intros i _ (_ & Hvb). apply Hfresh, Hvb.
+            intros b ofs Hb _. eauto.
+      -- intros b ofs Hb Hvb. split; assumption.
+Qed.
 
 End correctness.
 End Correctness.
